Updates.

FOL/Compute.lean
@@ -460,7 +460,7 @@ def LabeledTree.frontier
     else (List.ofFn (fun i : Fin order => (children i).frontier)).join
 
 
-inductive isDerivationNode
+inductive isParseNode
   (g : CFG) :
   LabeledTree (g.N ⊕ g.T) → Prop
 
@@ -469,25 +469,11 @@ inductive isDerivationNode
     (h : T.label.isLeft) :
     ¬ T.isLeaf →
     (T.label.getLeft h, (List.ofFn T.children).map label) ∈ g.P →
-    (∀ (i : Fin T.order), isDerivationNode g (T.children i)) →
-    isDerivationNode g T
+    (∀ (i : Fin T.order), isParseNode g (T.children i)) →
+    isParseNode g T
 
   | terminal
     (T : LabeledTree (g.N ⊕ g.T)) :
     T.label.isRight →
     T.isLeaf →
-    isDerivationNode g T
-
-
-
-
-theorem thm_2_1
-  (g : CFG)
-  (A : g.N)
-  (w : List (g.N ⊕ g.T))
-  (T : LabeledTree (g.N ⊕ g.T))
-  (h1 : isPartialDerivationTree g T) :
-  derives g [Sum.inl A] w :=
-  by
-  induction T
-  case node label order children ih
+    isParseNode g T
